proof/DDC/Language/SystemF2Data.v
@@ -60,5 +60,5 @@ Require Export DDC.Language.SystemF2Data.Progress.
 Require Export DDC.Language.SystemF2Data.Preservation.
 
 (* Big step evaluation, and conversion to small steps. *)
-Require Export DDC.Language.SystemF2.Eval.
+Require Export DDC.Language.SystemF2Data.Eval.
 
