proof/DDC/Language/SystemF2Store/StoreBind.v
@@ -1,0 +1,28 @@
+
+Require Export DDC.Language.SystemF2Store.StoreValue.
+Require Export DDC.Language.SystemF2Store.TyJudge.
+
+
+(* Store binding with a constructor tag and some storeable values *)
+Inductive sbind :=
+ | SObj : datacon -> list svalue -> sbind.
+
+
+Definition store  := list sbind.
+Hint Unfold store.
+
+
+(* Store binding is well typed under some data type defs and store environment. *)
+Inductive TYPEB (ds: defs) (se: stenv) : sbind -> ty -> Prop := 
+ | TyObj 
+   :  forall tc ks dc dcs tsFields tsParam svs xs
+   ,  DEFSOK ds
+   -> getTypeDef tc ds = Some (DefDataType tc ks dcs)
+   -> getDataDef dc ds = Some (DefData dc tsFields tc)
+   -> Forall2 (KIND nil) tsParam ks
+   -> Forall2 svalueOf   xs svs
+   -> Forall2 (TYPE ds nil nil se) xs (map (substTTs 0 tsParam) tsFields)
+   -> TYPEB ds se (SObj dc svs) (makeTApps (TCon tc) tsParam).
+Hint Constructors TYPEB.
+
+
