proof/DDC/Language/SystemF2Store/StoreValue.v
@@ -1,0 +1,98 @@
+
+Require Export DDC.Language.SystemF2Store.Exp.
+
+
+(********************************************************************)
+(* Storeable values are the ones that we can keep directly in 
+   store bindings *)
+Inductive svalue :=
+ | SLoc  : nat -> svalue
+ | SLAM  : exp -> svalue
+ | SLam  : ty  -> exp -> svalue.
+Hint Constructors svalue.
+
+
+Definition takeSValueOfExp (xx : exp) : option svalue :=
+ match xx with
+ | XLoc n    => Some (SLoc n)
+ | XLAM x    => Some (SLAM x)
+ | XLam t x  => Some (SLam t x)
+ | _         => None
+ end.
+
+
+Definition expOfSValue (s: svalue) : exp :=
+ match s with
+ | SLoc n    => XLoc n
+ | SLAM x    => XLAM x
+ | SLam t x  => XLam t x
+ end.
+
+
+Definition svalueOf (xx : exp) (sv : svalue) : Prop
+ := takeSValueOfExp xx = Some sv.
+
+
+(* There is an expression for every store value *)
+Lemma exp_from_svalue
+ : forall sv, exists v, svalueOf v sv.
+Proof.
+ intros.
+ destruct sv; unfold svalueOf.
+  exists (XLoc n). int.
+  exists (XLAM e). int.
+  exists (XLam t e). int.
+Qed.
+Hint Resolve exp_from_svalue.
+
+
+(* There is a store value for every expression value. *)
+Lemma svalue_from_value
+ : forall v, value v -> (exists sv, svalueOf v sv).
+Proof.
+ intros.
+ destruct v; nope; unfold svalueOf.
+  exists (SLoc  n).  eauto.
+  exists (SLAM  v).  eauto.
+  exists (SLam t v). eauto.
+Qed.
+Hint Resolve svalue_from_value.
+
+
+Lemma svalue_of_expOfSValue
+ : forall sv : svalue, svalueOf (expOfSValue sv) sv.
+Proof.
+ intros.
+ destruct sv; simpl; unfold svalueOf; simpl; auto.
+Qed.
+Hint Resolve svalue_of_expOfSValue.
+
+
+Lemma svalueOf_is_expOfSValue
+ :  forall v sv
+ ,  svalueOf v sv
+ -> v = expOfSValue sv.
+Proof.
+ intros.
+ inverts H.
+  destruct sv;
+   destruct v; try burn; simpl in *; inverts H1; auto.
+Qed.
+Hint Resolve svalueOf_is_expOfSValue.
+
+
+Lemma svalueOf_forall_expOfSValue
+ :  forall vs svs
+ ,  Forall2 svalueOf vs svs
+ -> vs = map expOfSValue svs.
+Proof.
+ intros.
+ induction H.
+  simpl. auto.
+  subst. simpl.
+  f_equal. 
+  eapply svalueOf_is_expOfSValue. auto.
+Qed.
+Hint Resolve svalueOf_forall_expOfSValue.
+
+
